thy/Primitive_Matchers/Common_Primitive_toString.thy
@@ -27,10 +27,12 @@ fun ipv4addr_wordinterval_toString :: "32 wordinterval \<Rightarrow> string" whe
 
 fun protocol_toString :: "protocol \<Rightarrow> string" where
   "protocol_toString (ProtoAny) = ''all''" |
-  "protocol_toString (Proto TCP) = ''tcp''" |
-  "protocol_toString (Proto UDP) = ''udp''" |
-  "protocol_toString (Proto ICMP) = ''icmp''" |
-  "protocol_toString (Proto (OtherProtocol protid)) = ''protocolid:''@string_of_nat protid"
+  "protocol_toString (Proto protid) = ( 
+  if protid = TCP then ''tcp'' else
+  if protid = UDP then ''udp'' else
+  if protid = ICMP then ''icmp'' else
+  if protid = SCTP then ''sctp'' else
+  ''protocolid:''@string_of_nat (unat protid))"
   
 
 
